@prefix dcosample:  <http://info.deepcarbon.net/sample/schema#> .
@prefix dco:     <http://info.deepcarbon.net/schema#> .
@prefix foaf:    <http://xmlns.com/foaf/0.1/> .
@prefix vivo:    <http://vivoweb.org/ontology/core#> .
@prefix vitro:   <http://vitro.mannlib.cornell.edu/ns/vitro/0.7#> .
@prefix dc:      <http://purl.org/dc/elements/1.1/> .
@prefix terms:   <http://purl.org/dc/terms/> .
@prefix dcterms:  <http://purl.org/dc/terms/> .
@prefix rdf:     <http://www.w3.org/1999/02/22-rdf-syntax-ns#> .
@prefix owl:     <http://www.w3.org/2002/07/owl#> .
@prefix rdfs:    <http://www.w3.org/2000/01/rdf-schema#> .
@prefix xsd:     <http://www.w3.org/2001/XMLSchema#> .
@prefix skos:    <http://www.w3.org/2004/02/skos/core#> .
@prefix obo:     <http://purl.obolibrary.org/obo/> .

<http://info.deepcarbon.net/sample/schema>
      a       owl:Ontology ;
      rdfs:label "DCO Sample Schema"@en-US ;
      dc:title "DCO Sample Schema"@en-US ;
      dc:creator <http://tw.rpi.edu/instances/PatrickWest> ;
      dc:contributor <http://tw.rpi.edu/instances/JohnErickson> ;
      dc:contributor <http://tw.rpi.edu/instances/StephanZednik> ;
      dc:contributor <http://tw.rpi.edu/instances/XiaogangMa> ;
      dc:contributor <http://tw.rpi.edu/instances/PeterFox> ;
      dc:contributor <http://tw.rpi.edu/instances/person/HaoZhong> ;
      dc:contributor <http://tw.rpi.edu/instances/person/AhmedEleish> ;
      dc:publisher <http://tw.rpi.edu/instances/TetherlessWorldConstellation> ;
      dc:date "2016-04-03"^^xsd:date ;
      dc:rights "This ontology is distributed under a Creative Commons Attribution License http://creativecommons.org/licenses/by/3.0/"@en-US;
      rdfs:comment  """
      This Deep Carbon Observatory (DCO) Ontology includes concepts and relationships that represent physical samples and repositories used within that
      are collected and maintained by members of the DCO Community
      """^^rdf:XMLLiteral .

dcosample:Sample
      a       owl:Class ;
      rdfs:label "Sample"@en-US ;
      rdfs:subClassOf dco:Object ;
      rdfs:subClassOf
              [ a       owl:Restriction ;
                owl:allValuesFrom xsd:string ;
                owl:onProperty vivo:identifier
              ] ;
      rdfs:comment  """
          a physical sample, obtained for observation(s)
      """^^rdf:XMLLiteral .

dcosample:SampleGroup
      a       owl:Class ;
      rdfs:label "Sample Group"@en-US ;
      rdfs:subClassOf dco:Object ;
      rdfs:subClassOf
              [ a       owl:Restriction ;
                owl:allValuesFrom dcosample:Sample ;
                owl:onProperty obo:BFO_0000051
              ] ;
      rdfs:comment  """
          A collection of samples usually with common attributes
      """^^rdf:XMLLiteral .

dcosample:SampleRepository
      a       owl:Class ;
      rdfs:label "Sample Repository"@en-US ;
      rdfs:subClassOf dco:Repository ;
      rdfs:comment  """
          A repository that contains physical samples
      """^^rdf:XMLLiteral .

dcosample:SampleType
      a       owl:Class ;
      rdfs:label "Sample Type"@en-US ;
      rdfs:subClassOf skos:Concept ;
      rdfs:comment  """
          vocabulary term representing types of samples
      """^^rdf:XMLLiteral .

dcosample:inSampleRepository
      a       owl:ObjectProperty ;
      rdfs:domain dcosample:Sample ;
      rdfs:label "in sample repository"@en-US ;
      rdfs:range dcosample:SampleRepository ;
      rdfs:comment  """
          A sample that is maintained within a repository of samples
      """^^rdf:XMLLiteral ;
      owl:inverseOf dcosample:includesSample .

dcosample:sampleCollectionComment
      a       owl:DatatypeProperty ;
      rdfs:domain dcosample:Sample ;
      rdfs:label "sample collection comment"@en-US ;
      rdfs:range rdf:XMLLiteral ;
      rdfs:comment  """
          Information about the act of collecting the sample
      """^^rdf:XMLLiteral .

dcosample:includesSampleType
      a       owl:ObjectProperty ;
      rdfs:domain dcosample:SampleGroup ;
      rdfs:label "includes sample type"@en-US ;
      rdfs:range dcosample:SampleType ;
      rdfs:comment  """
          Classification of samples that are in a particular group
      """^^rdf:XMLLiteral .

dcosample:hasSampleType
      a       owl:ObjectProperty ;
      rdfs:domain dcosample:Sample ;
      rdfs:label "has sample type"@en-US ;
      rdfs:range dcosample:SampleType ;
      rdfs:subPropertyOf vivo:hasSubjectArea ;
      rdfs:comment  """
          A formalized classification or annotation about a sample
      """^^rdf:XMLLiteral .

dcosample:sampleCollectionTime
      a       owl:DatatypeProperty ;
      rdfs:domain dcosample:Sample ;
      rdfs:label "sample collection time"@en-US ;
      rdfs:range xsd:dateTime ;
      rdfs:comment  """
          The sample was collected at a specific date and time
      """^^rdf:XMLLiteral .

dcosample:hasSampleAge
      a       owl:DatatypeProperty ;
      rdfs:domain dcosample:Sample ;
      rdfs:label "has sample age"@en-US ;
      rdfs:range xsd:string ;
      rdfs:comment  """
        The geologic age of a sample
      """^^rdf:XMLLiteral .

dcosample:includesSampleGroup
      a       owl:ObjectProperty ;
      rdfs:domain dcosample:SampleRepository ;
      rdfs:label "includes sample group"@en-US ;
      rdfs:range dcosample:SampleGroup ;
      rdfs:comment  """
          a sample repository can include collections of samples as well as individual samples
      """^^rdf:XMLLiteral .

dcosample:IGSN
      a       owl:DatatypeProperty ;
      rdfs:domain dcosample:Sample ;
      rdfs:label "IGSN"@en-US ;
      rdfs:range xsd:string ;
      rdfs:subPropertyOf vivo:identifier ;
      rdfs:comment  """
          IGSN stands for International Geo Sample Number. The IGSN is 9-character alphanumeric code that uniquely identifies samples taken from our natural environment (for example: rock specimens, water samples, sediment cores) as well as related sampling features (sites, stations, stratigraphic sections, etc.)
      """^^rdf:XMLLiteral .

dcosample:registeredBy
      a       owl:ObjectProperty ;
      rdfs:domain dcosample:Sample ;
      rdfs:label "registered by"@en-US ;
      rdfs:range foaf:Person ;
      rdfs:comment  """
          The person that registered the sample in a repository
      """^^rdf:XMLLiteral .

dcosample:fromSample
      a       owl:ObjectProperty ;
      rdfs:domain dcosample:Sample ;
      rdfs:label "from sample"@en-US ;
      rdfs:range dcosample:Sample ;
      rdfs:comment  """
          a physical sample that comes from a larger sample, such as a slice of a core sample
      """^^rdf:XMLLiteral .

dcosample:sampleFromFieldStudy
      a       owl:ObjectProperty ;
      rdfs:domain dcosample:Sample ;
      rdfs:label "sample from field study"@en-US ;
      rdfs:range dco:FieldStudy ;
      rdfs:comment  """
          A sample can be collected as part of a DCO funded field study
      """^^rdf:XMLLiteral ;
      owl:inverseOf dcosample:collectedSample .

dcosample:sampleGeographicArea
      a       owl:ObjectProperty ;
      rdfs:domain dcosample:Sample ;
      rdfs:label "sample geographic area"@en-US ;
      rdfs:comment  """
          The physical location from which a sample is collected
      """^^rdf:XMLLiteral .

dcosample:collectedSample
      a       owl:ObjectProperty ;
      rdfs:domain dco:FieldStudy ;
      rdfs:label "collected sample"@en-US ;
      rdfs:range dcosample:Sample ;
      rdfs:comment  """
        A sample was collected as part of a funded field study project
      """^^rdf:XMLLiteral ;
      owl:inverseOf dcosample:sampleFromFieldStudy .

dcosample:includesSample
      a       owl:ObjectProperty ;
      rdfs:domain dcosample:SampleRepository ;
      rdfs:label "includes sample"@en-US ;
      rdfs:range dcosample:Sample ;
      rdfs:comment  """
          a sample, such as a core sample, that is part of a sample repository
      """^^rdf:XMLLiteral ;
      owl:inverseOf dcosample:inSampleRepository .

