@prefix samfl:     <http://def.seegrid.csiro.au/ontology/om/sam-lite#> .
@prefix dcosample:  <http://info.deepcarbon.net/sample/schema#> .
@prefix vitro:   <http://vitro.mannlib.cornell.edu/ns/vitro/0.7#> .
@prefix rdf:     <http://www.w3.org/1999/02/22-rdf-syntax-ns#> .
@prefix dc:      <http://purl.org/dc/elements/1.1/> .
@prefix owl:     <http://www.w3.org/2002/07/owl#> .
@prefix dct:  <http://purl.org/dc/terms/> .
@prefix rdfs:    <http://www.w3.org/2000/01/rdf-schema#> .
@prefix vivo:    <http://vivoweb.org/ontology/core#> .
@prefix obo:     <http://purl.obolibrary.org/obo/> .
@prefix dco:     <http://info.deepcarbon.net/schema#> .
@prefix xsd:     <http://www.w3.org/2001/XMLSchema#> .
@prefix core:    <http://vivoweb.org/ontology/core#> .
@prefix skos:    <http://www.w3.org/2004/02/skos/core#> .
@prefix ero:     <http://purl.obolibrary.org/obo/> .
@prefix bibo:    <http://purl.org/ontology/bibo/> .
@prefix foaf:    <http://xmlns.com/foaf/0.1/> .

<http://info.deepcarbon.net/sample/schema>
      a       owl:Ontology ;
      rdfs:label "DCO Sample"@en-US .

dcosample:IGSNRegistration
      a       owl:Class ;
      rdfs:label "IGSN Registration"@en-US ;
      rdfs:comment  """
          information about the registration of an IGSN
      """^^rdf:XMLLiteral .

dcosample:igsnRegistrant
      a       owl:ObjectProperty ;
      rdfs:domain dcosample:IGSNRegistration ;
      rdfs:label "registered by"@en-US ;
      rdfs:range foaf:Person ;
      rdfs:comment  """
          registration of the sample to get igsn was done by a person
      """^^rdf:XMLLiteral .

dcosample:includesSampleType
      a       owl:ObjectProperty ;
      rdfs:domain dcosample:SampleGroup ;
      rdfs:label "includes sample type"@en-US ;
      rdfs:range dcosample:SampleType ;
      rdfs:comment  """
          A collection of samples includes samples of various types
      """^^rdf:XMLLiteral .

dcosample:hasSampleType
      a       owl:ObjectProperty ;
      rdfs:domain dcosample:Sample ;
      rdfs:label "has sample type"@en-US ;
      rdfs:range dcosample:SampleType ;
      rdfs:subPropertyOf core:hasSubjectArea ;
      rdfs:comment  """
          A sample classification or annotation
      """^^rdf:XMLLiteral .

dcosample:hasIGSNRegistration
      a       owl:ObjectProperty ;
      rdfs:domain samfl:SamplingFeature ;
      rdfs:label "has IGSN registration"@en-US ;
      rdfs:range dcosample:IGSNRegistration ;
      rdfs:comment  """
          information about the registration of the sampling feature such as registering, removing the registration, discarding the registration
      """^^rdf:XMLLiteral ;
      owl:inverseOf dcosample:registrationForSamplingFeature .

dcosample:registrationForSamplingFeature
      a       owl:ObjectProperty ;
      rdfs:range samfl:SamplingFeature ;
      rdfs:label "registration for sample"@en-US ;
      rdfs:domain dcosample:IGSNRegistration ;
      rdfs:comment  """
          The registration of the IGSN is for a given sampling feature
      """^^rdf:XMLLiteral ;
      owl:inverseOf dcosample:hasIGSNRegistration .

dcosample:includesSampleGroup
      a       owl:ObjectProperty ;
      rdfs:domain dcosample:SampleRepository ;
      rdfs:label "includes sample group"@en-US ;
      rdfs:range dcosample:SampleGroup ;
      rdfs:subPropertyOf core:hasPart ;
      rdfs:comment  """
          a sample repository can include collections of samples as well as individual samples
      """^^rdf:XMLLiteral ;
      owl:inverseOf dcosample:sampleGroupInRepository .

dcosample:sampleGroupInRepository
      a       owl:ObjectProperty ;
      rdfs:range dcosample:SampleRepository ;
      rdfs:label "sample group in"@en-US ;
      rdfs:domain dcosample:SampleGroup ;
      rdfs:subPropertyOf core:isPartOf ;
      rdfs:comment  """
          a collection of samples is in a sample repository
      """^^rdf:XMLLiteral ;
      owl:inverseOf dcosample:includesSampleGroup .

dcosample:SampleGroup
      a       owl:Class ;
      rdfs:label "Sample Group"@en-US ;
      rdfs:subClassOf dco:Object ;
      rdfs:subClassOf samfl:SamplingCollection ;
      rdfs:subClassOf
              [ a       owl:Restriction ;
                owl:allValuesFrom dcosample:Sample ;
                owl:onProperty ero:BFO_0000051
              ] ;
      rdfs:comment  """
          A collection of samples usually with common attributes
      """^^rdf:XMLLiteral .

dcosample:Sample
      a       owl:Class ;
      rdfs:label "Sample"@en-US ;
      rdfs:subClassOf dco:Object , samfl:Specimen ;
      rdfs:subClassOf
              [ a       owl:Restriction ;
                owl:allValuesFrom dco:Object ;
                owl:onProperty dct:isReferencedBy
              ] ;
      rdfs:subClassOf
              [ a       owl:Restriction ;
                owl:allValuesFrom xsd:string ;
                owl:onProperty core:description
              ] ;
      rdfs:subClassOf
              [ a       owl:Restriction ;
                owl:allValuesFrom bibo:Document ;
                owl:onProperty dco:isCitedBy
              ] ;
      rdfs:comment  """
          a physical sample, obtained for observation(s)
      """^^rdf:XMLLiteral .

dcosample:fromSample
      a       owl:ObjectProperty ;
      rdfs:domain dcosample:Sample ;
      rdfs:label "from sample"@en-US ;
      rdfs:range dcosample:Sample ;
      rdfs:comment  """
          a physical sample that comes from a larger sample, such as a slice of a core sample
      """^^rdf:XMLLiteral .

dcosample:igsn
      a       owl:DatatypeProperty ;
      rdfs:domain dcosample:Sample ;
      rdfs:label "IGSN"@en-US ;
      rdfs:range xsd:string ;
      rdfs:subPropertyOf core:identifier ;
      rdfs:comment  """
          IGSN stands for International Geo Sample Number. The IGSN is 9-character alphanumeric code that uniquely identifies samples taken from our natural environment (for example: rock specimens, water samples, sediment cores) as well as related sampling features (sites, stations, stratigraphic sections, etc.).
      """^^rdf:XMLLiteral .

dcosample:SampleType
      a       owl:Class ;
      rdfs:label "Sample Type"@en-US ;
      rdfs:subClassOf skos:Concept ;
      rdfs:comment  """
          vocabulary term representing types of samples
      """^^rdf:XMLLiteral .

dcosample:SampleRepository
      a       owl:Class ;
      rdfs:label "Sample Repository"@en-US ;
      rdfs:subClassOf dco:Repository ;
      rdfs:comment  """
          A repository where samples are maintained
      """^^rdf:XMLLiteral .

dcosample:sampleCurationPractice
      a       owl:DatatypeProperty ;
      rdfs:domain dcosample:SampleRepository ;
      rdfs:label "sample curation practice"@en-US ;
      rdfs:comment  """
          the curation practice employed for the sample repository
      """^^rdf:XMLLiteral ;
      rdfs:range rdf:XMLLiteral .

dcosample:sampleFromFieldStudy
      a       owl:ObjectProperty ;
      rdfs:domain dcosample:Sample ;
      rdfs:label "sample from field study"@en-US ;
      rdfs:range dco:FieldStudy ;
      rdfs:comment  """
          A sample can be collected as part of a DCO funded field study
      """^^rdf:XMLLiteral ;
      owl:inverseOf dcosample:collectedSample .

dcosample:collectedSample
      a       owl:ObjectProperty ;
      rdfs:domain dco:FieldStudy ;
      rdfs:label "collected sample"@en-US ;
      rdfs:range dcosample:Sample ;
      rdfs:comment  """
      As part of a field study project a sample, such as a core or rock sample, is collected
      """^^rdf:XMLLiteral ;
      owl:inverseOf dcosample:sampleFromFieldStudy .

dcosample:includesSample
      a       owl:ObjectProperty ;
      rdfs:domain dcosample:SampleRepository ;
      rdfs:label "includes sample"@en-US ;
      rdfs:range dcosample:Sample ;
      rdfs:subPropertyOf core:hasPart ;
      rdfs:comment  """
          a sample, such as a core sample, that is part of a sample repository
      """^^rdf:XMLLiteral ;
      owl:inverseOf dcosample:inSampleRepository .

dcosample:inSampleRepository
      a       owl:ObjectProperty ;
      rdfs:domain dcosample:Sample ;
      rdfs:label "in sample repository"@en-US ;
      rdfs:range dcosample:SampleRepository ;
      rdfs:subPropertyOf core:isPartOf ;
      rdfs:comment  """
      A sample, such as a core or rock sample, is included in, or is part of, a sample repository
      """^^rdf:XMLLiteral ;
      owl:inverseOf dcosample:includesSample .

dcosample:isMemberOf
      a       owl:ObjectProperty ;
      rdfs:domain samfl:SamplingFeature ;
      rdfs:label "member of" ;
      rdfs:range samfl:SamplingCollection ;
      rdfs:comment """
          the sampling feature is a member of a sampling collection
      """^^rdf:XMLLiteral ;
      owl:inverseOf samfl:member .

