@prefix dco:     <http://info.deepcarbon.net/schema#> .
@prefix rdf:     <http://www.w3.org/1999/02/22-rdf-syntax-ns#> .
@prefix owl:     <http://www.w3.org/2002/07/owl#> .
@prefix rdfs:    <http://www.w3.org/2000/01/rdf-schema#> .
@prefix dc:      <http://purl.org/dc/terms/> .
@prefix vivo:    <http://vivoweb.org/ontology/core#> .
@prefix prov:    <http://www.w3.org/ns/prov#> .
@prefix bibo:    <http://purl.org/ontology/bibo/> .
@prefix xsd:     <http://www.w3.org/2001/XMLSchema#> .
@prefix skos:    <http://www.w3.org/2004/02/skos/core#> .
@prefix type:    <http://info.deepcarbon.net/schema/type#> .

##### Data Type Ontology
<http://info.deepcarbon.net/schema/type>
      a       owl:Ontology ;
      rdfs:label "Data Type Ontology"@en-US ;
      dc:title "Data Type Ontology"@en-US ;
      dc:creator <http://tw.rpi.edu/instances/XiaogangMa>;
      dc:contributor <http://tw.rpi.edu/instances/JohnErickson> ;
      dc:contributor <http://tw.rpi.edu/instances/PatrickWest> ;
      dc:contributor <http://tw.rpi.edu/instances/StephanZednik> ;
      dc:contributor <http://tw.rpi.edu/instances/PeterFox> ;
      dc:publisher <http://tw.rpi.edu/instances/TetherlessWorldConstellation> ;
      dc:date "2015-11-02"^^xsd:date ;
      dc:rights "This ontology is distributed under a Creative Commons Attribution License http://creativecommons.org/licenses/by/3.0/"@en-US;
      rdfs:comment  """
      The Data Type Ontology represents concepts and relationships for the formal specification of data types. 
	  In this ontology a data type is regarded as the representation of particular qualities or features that a 
	  group of datasets share. The ontology allows people to add domain specific meanings to a data type, to register 
	  the data type as an object in a data repository, and to annotate a resource by associating it with one 
	  or more data types. 
      """^^rdf:XMLLiteral .
##### DataTypes
type:DataType
      a       owl:Class ;
      rdfs:comment  """
      A data type is often treated as a purely syntactic
      label associated with a variable when it is declared, such as
      integer, float, boolean, character, and string, etc. Such
      definitions of 'data type' do not give any semantic meaning to the
      data types. In the context of this ontology, a data type can
      include more meaning beyond the syntax, such as who created the
      data type, the source standard that the data type derives from,
      the operations that can be done on datasets of that data type, and
      typical scientific domains, software programs and/or instruments
      that use the data type, etc. The intent is that any humans or
      machines that when they encounter that data type can quickly
      'understand' or be in a situation to at least 'process' details
      within the dataset without even downloading that dataset.
      """^^rdf:XMLLiteral ;
      rdfs:label "Data Type"@en-US ;
      rdfs:subClassOf dco:Object , prov:Entity ;
      skos:definition "A data type is the representation of particular qualities or features that a group of datasets share." .

type:DataTypeParameter
      a       owl:Class ;
      rdfs:comment  """
      The data type includes a set of variables that define its usage. A
      user can find a datatype and know to expect these parameters to be
      a part of the dataset that the data type is associated with.
      Another use is that someone can find a datatype that a variable is
      a part of and then find additional datasets that this datatype is
      associated with.
      """^^rdf:XMLLiteral ;
      rdfs:label "DataType Parameter"@en-US ;
      rdfs:subClassOf dco:Object , prov:Entity ;
      skos:definition "An input variable of a data type." .

type:hasDataTypeParameter
      a       owl:ObjectProperty ;
      rdfs:comment "Link a DataType with variables that make up the DataType" ;
      rdfs:domain dco:DataType ;
      rdfs:label "has parameter" ;
      rdfs:range dco:DataTypeParameter .

type:hasUnit
      a       owl:DatatypeProperty ;
      rdfs:comment  """
      Annotate the unit, e.g. meter, degree, dollar, etc. of a parameter.
      """^^rdf:XMLLiteral ;
      rdfs:domain dco:DataTypeParameter ;
      rdfs:label "has unit" ;
      rdfs:range xsd:string .

type:expectedUses
      a       owl:DatatypeProperty ;
      rdfs:comment  """
      describes any additional constraints, comments or notes about a
      data type.
      """^^rdf:XMLLiteral ;
      rdfs:domain dco:DataType ;
      rdfs:label "expected uses" ;
      rdfs:range xsd:string .

type:dataTypeSubjectArea
      a       owl:ObjectProperty ;
      rdfs:comment  """
      Associates a data type with the different defined domains of
      knowledge and skill within the Deep Carbon Observatory community.
      """^^rdf:XMLLiteral ;
      rdfs:domain dco:DataType ;
      rdfs:label "has data type subject area" ;
      rdfs:range skos:Concept ;
      rdfs:subPropertyOf vivo:hasSubjectArea .

type:createdAtTime
      a       owl:DatatypeProperty ;
      rdfs:comment  """
      Part of the provenance of a data type, at what time was the data
      type created.
      """^^rdf:XMLLiteral ;
      rdfs:domain dco:DataType ;
      rdfs:label "created at time" ;
      rdfs:range xsd:dateTime .

type:sourceStandard
      a       owl:ObjectProperty ;
      rdfs:comment  """
      A data type may be derived from one or more universally or widely
      accepted, agreed upon, or established means of determining what
      something should be.
      """^^rdf:XMLLiteral ;
      rdfs:domain dco:DataType ;
      rdfs:label "has source standard" ;
      rdfs:range bibo:Standard ;
      rdfs:subPropertyOf prov:wasDerivedFrom .

type:sourceDataType
      a       owl:ObjectProperty ;
      rdfs:comment  """
      Part of the provenance of a data type, a data type may be derived
      from one or more existing data types.  For example, a data type
      can add one or more variables to an existing data type making it a
      new data type.
      """^^rdf:XMLLiteral ;
      rdfs:domain dco:DataType ;
      rdfs:label "has source data type" ;
      rdfs:range dco:DataType ;
      rdfs:subPropertyOf prov:wasDerivedFrom .

type:lastModifiedAtTime
      a       owl:DatatypeProperty ;
      rdfs:comment  """
      Part of the provenance of a data type this property represents
      the most recent time that a data type was modified
      """^^rdf:XMLLiteral ;
      rdfs:domain dco:DataType ;
      rdfs:label "last modified at time" ;
      rdfs:range xsd:dateTime .